coq/Logic/Prop/Sound.v
@@ -1,6 +1,9 @@
+Require Import List.
+
 Require Import Logic.Prop.Syntax.
 Require Import Logic.Prop.Context.
 Require Import Logic.Prop.Proof.
+Require Import Logic.Prop.Semantics.
 Require Import Logic.Prop.Entails.
 
 (* If G :- p has a proof then the semantics entailment G ::- p holds            *)
@@ -18,3 +21,19 @@ Proof.
   - apply entReduct, IH.
 Qed.
 
+
+(* Every tautology is true under any truth assignment                           *)
+Lemma tautologyIsTrue1 : forall (v:Type) (f:v -> bool) (p:P v) (e:nil :- p),
+  eval f p = true.
+Proof.
+  intros v f p e. apply Soundness in e. apply e.
+  intros q H. inversion H.
+Qed.
+
+(* Every tautology is true under any valuation                                  *)
+Lemma tautologyIsTrue2 : forall (v:Type) (f:P v -> bool) (p:P v) (e:nil :- p),
+  Valuation f -> f p = true.
+Proof.
+  intros v f p e Hf. rewrite valIsEval. 2: apply Hf.
+  apply tautologyIsTrue1, e.
+Qed.
